finished stackmachine

Cpdt/StackMachine.v
@@ -1,3 +1,173 @@
-Require Import Bool Arith List.
-Require Export CpdtTactics.
+Require Import Bool Arith List CpdtTactics.
+Set Implicit Arguments.
+Set Asymmetric Patterns.
 
+Inductive binop : Set :=
+| Plus : binop
+| Times : binop.
+
+Inductive exp : Set :=
+| Const : nat -> exp
+| Binop : binop -> exp -> exp -> exp.
+
+Definition binopDenote (b : binop) : nat -> nat -> nat :=
+  match b with
+  | Plus => plus
+  | Times => mult
+  end.
+
+Fixpoint expDenot (e : exp) : nat :=
+  match e with
+  | Const n => n
+  | Binop b e1 e2 => (binopDenote b) (expDenot e1) (expDenot e2)
+  end.
+
+Eval simpl in expDenot (Const 42).
+Eval simpl in expDenot (Binop Plus (Const 42) (Const 1)).
+
+(* target language *)
+
+Inductive instr : Set :=
+| iConst : nat -> instr
+| iBinop : binop -> instr.
+
+Definition prog := list instr.
+Definition stack := list nat.
+
+Definition instrDenote (i : instr) (s : stack) : option stack :=
+  match i with
+  | iConst n => Some (n :: s)
+  | iBinop b =>
+    match s with
+    | arg1 :: arg2 :: s' => Some ((binopDenote b) arg1 arg2 :: s')
+    | _ => None
+    end
+  end.
+
+Fixpoint progDenot (p : prog) (s : stack) : option stack :=
+  match p with
+  | nil => Some s
+  | i :: p' =>
+    match instrDenote i s with
+    | None => None
+    | Some s' => progDenot p' s'
+    end
+  end.
+
+Fixpoint compile (e : exp) : prog :=
+  match e with
+  | Const n => iConst n :: nil
+  | Binop b e1 e2 =>
+    compile e2 ++ compile e1 ++ iBinop b :: nil
+  end.
+
+Eval simpl in compile (Const 42).
+Eval simpl in compile (Binop Plus (Const 2) (Const 2)).
+
+Theorem compiler_correct : forall e, progDenot (compile e) nil = Some (expDenot e :: nil).
+Proof.
+  induction e.
+  +  simpl. reflexivity.
+  + simpl.
+Abort.
+
+Lemma compiler_correct' : forall e p s,
+    progDenot (compile e ++ p) s = progDenot p (expDenot e :: s).
+Proof.
+  induction e.
+  + intros. unfold compile. unfold expDenot.
+    unfold progDenot at 1. simpl. fold progDenot.
+    reflexivity.
+  + intros. unfold compile. fold compile.
+    unfold expDenot. fold expDenot.
+    rewrite app_assoc_reverse. rewrite IHe2.
+    rewrite app_assoc_reverse. rewrite IHe1.
+    unfold progDenot at 1. simpl. fold progDenot.
+    reflexivity.
+Qed.
+
+Print compiler_correct'.
+
+Lemma compile_correct' :
+  forall e s p, progDenot (compile e ++ p) s = progDenot p (expDenot e :: s).
+Proof.
+  induction e; crush.
+Qed.
+
+Theorem compiler_correct : forall e, progDenot (compile e) nil = Some (expDenot e :: nil).
+Proof.
+  intros. Check app_nil_end.
+  rewrite (app_nil_end (compile e)).
+  rewrite compiler_correct'. reflexivity.
+Qed.
+
+Inductive type : Set :=
+| Nat : type
+| Bool : type.
+
+Inductive tbinop : type -> type -> type -> Set :=
+| TPlus : tbinop Nat Nat Nat
+| TTimes : tbinop Nat Nat Nat
+| TEq t : tbinop t t Bool
+| TLt : tbinop Nat Nat Bool.
+
+Inductive texp : type -> Set :=
+| TNConst : nat -> texp Nat
+| TBConst : bool -> texp Bool
+| TBinop t t1 t2 : tbinop t1 t2 t -> texp t1 -> texp t2 -> texp t.
+
+Definition typeDenote (t : type) : Set :=
+  match t with
+  | Nat => nat
+  | Bool => bool
+  end.
+
+Definition tbinopDenote arg1 arg2 res (b : tbinop arg1 arg2 res) :
+  typeDenote arg1 -> typeDenote arg2 -> typeDenote res :=
+  match b with
+  | TPlus => plus
+  | TTimes => mult
+  | TEq Nat => beq_nat
+  | TEq Bool => eqb
+  | TLt => leb
+  end.
+
+Fixpoint texpDenote t (e : texp t) : typeDenote t :=
+  match e with
+  | TNConst n => n
+  | TBConst b => b
+  | TBinop _ _ _ b e1 e2 => (tbinopDenote b) (texpDenote e1) (texpDenote e2)
+  end.
+
+Eval simpl in texpDenote (TNConst 42).
+
+Definition tstack := list type.
+
+Inductive tinstr : tstack -> tstack -> Set :=
+| TiNConst s : nat -> tinstr s (Nat :: s)
+| TiBConst b : bool -> tinstr b (Bool :: b)
+| TiBinop arg1 arg2 res s :
+    tbinop arg1 arg2 res -> tinstr (arg1 :: arg2 :: s) (res :: s).
+
+Inductive tprog : tstack -> tstack -> Set :=
+| TNil s : tprog s s
+| TCons s1 s2 s3 : tinstr s1 s2 -> tprog s2 s3 -> tprog s1 s3.
+
+
+Fixpoint vstack (ts : tstack) : Set :=
+  match ts with
+  | nil => unit
+  | t :: ts' => typeDenote t * vstack ts'
+  end%type.
+
+Definition tinstrDenote ts ts' (i : tinstr ts ts') : vstack ts -> vstack ts' :=
+  match i with
+  | TiNConst _ n => fun s => (n, s)
+  | TiBConst _ b => fun s => (b, s)
+  | TiBinop _ _ _ _ b =>
+    fun s => let '(arg1, (arg2, s')) := s in
+                   ((tbinopDenote b) arg1 arg2, s')
+               end.
+
+
+                          
